Extension.thy
@@ -4,6 +4,8 @@ theory Extension
   imports Substitutions
 begin
 
+subsection \<open> Expressions \<close>
+
 syntax 
   "_aext"      :: "logic \<Rightarrow> svid \<Rightarrow> logic" (infixl "\<up>" 80)
   "_ares"      :: "logic \<Rightarrow> svid \<Rightarrow> logic" (infixl "\<down>" 80)
@@ -34,12 +36,28 @@ lemma aext_ares: "\<lbrakk> mwb_lens a; (- $a) \<sharp> P \<rbrakk> \<Longrighta
   by (auto simp add: expr_defs fun_eq_iff lens_create_def)
 
 lemma expr_pre [simp]: "e\<^sup>< (s\<^sub>1, s\<^sub>2) = (e)\<^sub>e s\<^sub>1"
-  by (simp add: subst_aext_def subst_app_def)
+  by (simp add: subst_ext_def subst_app_def)
 
 lemma expr_post [simp]: "e\<^sup>> (s\<^sub>1, s\<^sub>2) = (@e)\<^sub>e s\<^sub>2"
-  by (simp add: subst_aext_def subst_app_def)
+  by (simp add: subst_ext_def subst_app_def)
 
 lemma unrest_aext_expr_lens [unrest]: "\<lbrakk> mwb_lens x; x \<bowtie> a \<rbrakk> \<Longrightarrow> $x \<sharp> (P \<up> a)"
   by (expr_simp add: lens_indep.lens_put_irr2)
+
+subsection \<open> Substitutions \<close>
+
+definition subst_aext :: "'a subst \<Rightarrow> ('a \<Longrightarrow> 'b) \<Rightarrow> 'b subst"
+  where [expr_defs]: "subst_aext \<sigma> x = (\<lambda> s. put\<^bsub>x\<^esub> s (\<sigma> (get\<^bsub>x\<^esub> s)))"
+
+definition subst_ares :: "'b subst \<Rightarrow> ('a \<Longrightarrow> 'b) \<Rightarrow> 'a subst"
+  where [expr_defs]: "subst_ares \<sigma> x = (\<lambda> s. get\<^bsub>x\<^esub> (\<sigma> (create\<^bsub>x\<^esub> s)))"
+
+syntax 
+  "_subst_aext" :: "logic \<Rightarrow> svid \<Rightarrow> logic" (infixl "\<up>\<^sub>s" 80)
+  "_subst_ares" :: "logic \<Rightarrow> svid \<Rightarrow> logic" (infixl "\<down>\<^sub>s" 80)
+
+translations
+  "_subst_aext P a" == "CONST subst_aext P a"
+  "_subst_ares P a" == "CONST subst_ares P a"
 
 end
